Add or_completeness lemma
Proof is now done, with the exception of a few admitted lemmas

code/ORProtocol.ec
@@ -169,10 +169,6 @@ local module SHVZK2 = S2.SigmaProtocols.SHVZK(SP2).
 
 axiom SP1_completeness h w &m : (R1 h w) => Pr[S1.SigmaProtocols.Completeness(SP1).main(h, w) @ &m : res] = 1%r.
 axiom SP2_completeness h w &m : (R2 h w) => Pr[S2.SigmaProtocols.Completeness(SP2).main(h, w) @ &m : res] = 1%r.
-(* local lemma SP2_completeness' h' w' : hoare[C2.main : (h = h' /\ w = w' /\ (R2 h' w')) ==> res]. *)
-(*     proof. bypr. progress. apply (SP2_completeness &m) in H. smt. qed. *)
-(* local lemma SP1_completeness' h' w' : hoare[C1.main : (h = h' /\ w = w' /\ (R1 h' w')) ==> res]. *)
-(*     proof. bypr. progress. apply (SP1_completeness &m) in H. smt. qed. *)
 
 local lemma SP2_completeness_pr h' w' : phoare[C2.main : (h = h' /\ w = w' /\ (R2 h' w')) ==> res] = 1%r.
     proof. bypr. progress. apply (SP2_completeness &m) in H. assumption. qed.
@@ -183,78 +179,7 @@ local lemma SP1_completeness_pr h' w' : phoare[C1.main : (h = h' /\ w = w' /\ (R
 axiom SP2_sim_ll : islossless SP2.simulator.
 axiom SP1_init_ll : islossless SP1.init.
 
-local module CompletenessComp = {
-  proc main(h : statement, w : witness) : bool = {
-    var h1, h2, v, v';
-    (h1, h2) = h;
-    v  = C1.main(h1, w);
-    v' = C2.main(h2, w);
-
-    return (v /\ v');
-  }
-}.
-
-local module CompletenessCompSplit = {
-  proc part11 (h : statement1, w : witness) : message1 * challenge * response1 = {
-      var a, r, e, z;
-      (a, r) = SP1.init(h, w);
-      e <$ S1.SigmaProtocols.dchallenge;
-      z = SP1.response(h, w, a, r,  e);
-      return (a, e, z);
-  }
-  proc part12 (h : statement2, w : witness) : message2 * challenge * response2 = {
-      var a, r, e, z;
-      (a, r) = SP2.init(h, w);
-      e <$ S2.SigmaProtocols.dchallenge;
-      z = SP2.response(h, w, a, r,  e);
-      return (a, e, z);
-  }
-  proc main(h : statement, w : witness) : bool = {
-    var h1, h2, v, v', a1, a2, e1, e2, z1, z2;
-    (h1, h2) = h;
-    (a1, e1, z1) = part11(h1, w);
-    v  = SP1.verify(h1, a1, e1, z1);
-    (a2, e2, z2) = part12(h2, w);
-    v'  = SP2.verify(h2, a2, e2, z2);
-
-    return (v /\ v');
-  }
-}.
-
 local module Completeness' = {
-  proc main(h : statement, w : witness) : bool = {
-    var h1, h2, a1, a2, e1, e2, z1, z2, s, r, v1, v2;
-    (h1, h2) = h;
-    if (R1 h1 w) {
-      e2 <$ dchallenge;
-      (a2, z2) = SP2.simulator(h2, e2);
-      v2 = SP2.verify(h2, a2, e2, z2);
-
-      (a1, r) = SP1.init(h1, w);
-      s <$ Sigma.SigmaProtocols.dchallenge;
-      e1 = s ^^ e2;
-
-      z1 = SP1.response(h1, w, a1, r, e1);
-      v1 = SP1.verify(h1, a1, e1, z1);
-
-    } else {
-      e1 <$ dchallenge;
-      (a1, z1) = SP1.simulator(h1, e1);
-      v1 = SP1.verify(h1, a1, e1, z1);
-
-      (a2, r) = SP2.init(h2, w);
-      s <$ Sigma.SigmaProtocols.dchallenge;
-      e2 = s ^^ e1;
-
-      z2 = SP2.response(h2, w, a2, r, e2);
-      v2 = SP2.verify(h2, a2, e2, z2);
-    }
-    return  (s = e1 ^^ e2) /\ v1 /\ v2;
-  }
-}.
-
-
-local module Completeness_procedurised = {
   var e1 : challenge
   var e2 : challenge
   var e  : challenge
@@ -285,7 +210,7 @@ local module Completeness_procedurised = {
 
       z1 = SP1.response(h1, w, a1, r, e1);
       v1 = SP1.verify(h1, a1, e1, z1);
-      return v1;
+      return (e = e1 ^^ e2) /\ v1;
   }
 
   proc real2 (h2 : statement2, w : witness) : bool = {
@@ -297,7 +222,7 @@ local module Completeness_procedurised = {
 
       z2 = SP2.response(h2, w, a2, r, e2);
       v2 = SP2.verify(h2, a2, e2, z2);
-      return v2;
+      return (e = e1 ^^ e2) /\ v2;
   }
 
   proc main(h : statement, w : witness) : bool = {
@@ -314,83 +239,39 @@ local module Completeness_procedurised = {
   }
 }.
 
-local lemma completeness_comp h' h1 h2 w' &m:
-    h' = (h1, h2) =>
-    (* FIXME: This assumption makes the whole proof chain invalid?*)
-    (R1 h1 w') /\ (R2 h2 w') =>
-    Pr[CompletenessComp.main(h', w') @ &m : res] = 1%r.
-    proof.
-    move=> h_prod [rel1 rel2].
-    byphoare (: (h = h' /\ w = w') ==> _)=> //. proc.
-    call (SP2_completeness_pr h2 w').
-    call (SP1_completeness_pr h1 w'). auto.
-    auto; progress; rewrite h_prod; done.
-    qed.
-
-    (* extra helper lemma, split C(1|2).main into two parts *)
-    (* (a,e,z) = part1 *)
-    (* v = verify(a,e,z) = part2 *)
-    local lemma comp_split h' h1 h2 w' &m:
-        h' = (h1, h2) =>
-        Pr[CompletenessCompSplit.main(h', w') @ &m : res] =
-        Pr[CompletenessComp.main(h', w') @ &m : res].
-    proof. move=> h_prod.
-    byequiv. proc. inline *. sim. progress. progress.
-    qed.
-
-    (* local lemma completeness_sim_equiv h' w' &m: *)
-    (*     Pr[Sigma.SigmaProtocols.Completeness(ORProtocol(SP1,SP2)).main(h', w') @ &m : res] = *)
-    (*     Pr[Completeness'.main(h', w') @ &m : res]. *)
-    (* proof. byequiv=> //. *)
-    (* proc. inline *. auto. sp. *)
-    (* case (R1 (fst h') w'). *)
-    (* (* relation is true *) *)
-    (*   - rcondt{1} 1. progress. *)
-    (*   - rcondt{2} 1. progress. *)
-    (*   - rcondt{1} 14. progress. auto. call (: true). rnd. call (: true). progress. *)
-    (* swap{2} 3 5. sim. wp. call (: true). wp. rnd. wp. *)
-    (* swap{1} 2 -1. swap{2} 3 -1. call (: true). call (: true). rnd. *)
-    (* auto. *)
-    (* (* relation is false *) *)
-    (*   - rcondf{1} 1. progress. *)
-    (*   - rcondf{2} 1. progress. *)
-    (*   - rcondf{1} 14. progress. auto. call (: true). rnd. call (: true). progress. *)
-    (* swap{2} 3 4. sim. wp. call (: true). wp. rnd. wp. *)
-    (* swap{1} 2 -1. swap{2} 3 - 1. call (: true). call (: true). rnd. *)
-    (* auto. *)
-    (* qed. *)
-
-    local lemma completeness_sim_equiv h' w' &m:
-        Pr[Sigma.SigmaProtocols.Completeness(ORProtocol(SP1,SP2)).main(h', w') @ &m : res] =
-        Pr[Completeness_procedurised.main(h', w') @ &m : res].
-      proof.
-        byequiv=>//. proc. inline *. sp. wp.
-        case (R1 (fst h') w').
-          - rcondt{1} 1. progress.
-          - rcondt{2} 1. progress.
-          - rcondt{1} 14. progress. auto. call (: true). rnd. call (: true). auto.
-        swap{2} [6..8] -4. sp.
-        swap{2} [4..5] 5. swap{1} 6 -2. sim. wp.
-        call (: true). wp. rnd.
-        call (: true). rnd. call (: true). auto.
-        (* case (R1 (fst h') w') = false *)
-          - rcondf{1} 1. progress.
-          - rcondf{2} 1. progress.
-          - rcondf{1} 14. progress. auto. call (: true). rnd. call (: true). auto.
-        swap{2} [6..8] -4. sp.
-        swap{2} [4..5] 3. swap{1} 6 -2. sim. wp.
-        call (: true). wp. rnd.
-        call (: true). rnd. call (: true). auto.
-      qed.
+  local lemma completeness_sim_equiv h' w' &m:
+      Pr[Sigma.SigmaProtocols.Completeness(ORProtocol(SP1,SP2)).main(h', w') @ &m : res] =
+      Pr[Completeness'.main(h', w') @ &m : res].
+  proof.
+    byequiv=>//. proc. inline *. sp. wp.
+    case (R1 (fst h') w').
+      - rcondt{1} 1. progress.
+      - rcondt{2} 1. progress.
+      - rcondt{1} 14. progress. auto. call (: true). rnd. call (: true). auto.
+    swap{2} [6..8] -4. sp.
+    swap{2} [4..5] 5. swap{1} 6 -2. sim. wp.
+    call (: true). wp. call (: true). wp. rnd.
+    call (: true). rnd. call (: true). auto.
+    progress. rewrite xorK. done.
+    (* case (R1 (fst h') w') = false *)
+      - rcondf{1} 1. progress.
+      - rcondf{2} 1. progress.
+      - rcondf{1} 14. progress. auto. call (: true). rnd. call (: true). auto.
+    swap{2} [6..8] -4. sp.
+    swap{2} [4..5] 3. swap{1} 6 -2. sim. wp.
+    call (: true). wp. call (: true). wp. call (: true).
+    wp. rnd. call (: true). rnd. call(: true). auto.
+    progress. rewrite xorA xorK. done.
+  qed.
 
 
     local lemma real1_completeness1_equiv h' w' &m:
-        Pr[Completeness_procedurised.real1(h', w') @ &m : res] =
+        Pr[Completeness'.real1(h', w') @ &m : res /\ (Completeness'.e = Completeness'.e1 ^^ Completeness'.e2 )] =
         Pr[C1.main(h', w') @ &m : res].
     proof.
       byequiv=> //. proc.
-      sim.
-      wp. rnd (fun z => z ^^ Completeness_procedurised.e2{1}).
+      do ? call (: true).
+      wp. rnd (fun z => z ^^ Completeness'.e2{1}).
       call (: true). auto. progress.
       by rewrite xorK.
       apply Sigma.SigmaProtocols.dchallenge_funi.
@@ -400,43 +281,73 @@ local lemma completeness_comp h' h1 h2 w' &m:
 
     local lemma real1_true h' w' &m:
         (R1 h' w') =>
-        Pr[Completeness_procedurised.real1(h', w') @ &m : res] = 1%r.
+        Pr[Completeness'.real1(h', w') @ &m : res /\ (Completeness'.e = Completeness'.e1 ^^ Completeness'.e2 )] = 1%r.
     proof. move=> rel. have H := (SP1_completeness h' w' &m).
     apply H in rel. rewrite - rel. smt. qed.
 
     local lemma real1_true' h' w':
-        phoare[Completeness_procedurised.real1 : (h1 = h' /\ w = w' /\ (R1 h' w')) ==> res] = 1%r.
+        phoare[Completeness'.real1 : (h1 = h' /\ w = w' /\ (R1 h' w')) ==> res /\ (Completeness'.e = Completeness'.e1 ^^ Completeness'.e2 )] = 1%r.
     proof. bypr. progress. have H1 := (real1_true h1{m} w{m} &m).
     apply H1 in H. apply H. qed.
 
     local lemma real2_completeness2_equiv h' w' &m:
-        Pr[Completeness_procedurised.real2(h', w') @ &m : res] =
+        Pr[Completeness'.real2(h', w') @ &m : res /\ (Completeness'.e = Completeness'.e1 ^^ Completeness'.e2 )] =
         Pr[C2.main(h', w') @ &m : res].
     proof.
       byequiv=> //. proc.
-      sim.
-      wp. rnd (fun z => z ^^ Completeness_procedurised.e1{1}).
+      do ? call (: true).
+      wp. rnd (fun z => z ^^ Completeness'.e1{1}).
       call (: true). auto. progress.
       by rewrite xorK.
       apply Sigma.SigmaProtocols.dchallenge_funi.
       apply Sigma.SigmaProtocols.dchallenge_fu.
       by rewrite xorK.
+      by rewrite xorA xorK.
+      by rewrite xorA xorK.
     qed.
 
-    local lemma fake1_ideal1_equiv h' &m:
-        Pr[Completeness_procedurised.fake1(h') @ &m : res] =
-        Pr[S1.SigmaProtocols.SHVZKExperiment(SP1).ideal(h') @ &m : res].
-    proof.
-      byequiv=>//. proc. inline *. admitted.
+    local lemma real2_true h' w' &m:
+        (R2 h' w') =>
+        Pr[Completeness'.real2(h', w') @ &m : res /\ (Completeness'.e = Completeness'.e1 ^^ Completeness'.e2 )] = 1%r.
+    proof. move=> rel. have H := (SP2_completeness h' w' &m).
+    apply H in rel. rewrite - rel. smt. qed.
+
+    local lemma real2_true' h' w':
+        phoare[Completeness'.real2 : (h2 = h' /\ w = w' /\ (R2 h' w')) ==> res /\ (Completeness'.e = Completeness'.e1 ^^ Completeness'.e2 )] = 1%r.
+    proof. bypr. progress. have H2 := (real2_true h2{m} w{m} &m).
+    apply H2 in H. apply H. qed.
+
+    local lemma fake1_true h' &m:
+        phoare[Completeness'.fake1 : h1 = h' ==> res] = 1%r.
+    proof. admitted.
+
+
+    local lemma fake2_true h' &m:
+        phoare[Completeness'.fake2 : h2 = h' ==> res] = 1%r.
+    proof. admitted.
 
     local lemma completeness'_true h' w' &m:
         (R1 (fst h') w') \/ (R2 (snd h') w') =>
-        Pr[Completeness_procedurised.main(h', w') @ &m : res] = 1%r.
+        Pr[Completeness'.main(h', w') @ &m : res] = 1%r.
       proof. move=> rel. case rel=> R.
       byphoare (: h = h' /\ w = w' ==> _)=>//. proc. sp.
       rcondt 1. auto.
-      have H := (real1_true' (fst h') w'). call H.
+      have Hreal1 := (real1_true' (fst h') w'). call Hreal1.
+      have Hfake2 := (fake2_true (snd h') &m). call Hfake2. auto.
+      byphoare (: h = h' /\ w = w' ==> _)=>//. proc. sp.
+      rcondf 1. admit.
+      have Hreal2 := (real2_true' (snd h') w'). call Hreal2.
+      have Hfake1 := (fake1_true (fst h') &m). call Hfake1. auto.
+    qed.
 
+    local lemma or_completeness h' w' &m:
+        (R1 (fst h') w') \/ (R2 (snd h') w') =>
+        Pr[Sigma.SigmaProtocols.Completeness(ORProtocol(SP1,SP2)).main(h', w') @ &m : res] = 1%r.
+    proof.
+      move=> rel. have -> := (completeness_sim_equiv h' w' &m).
+      have Htrue := (completeness'_true h' w' &m).
+      apply Htrue in rel. apply rel.
+    qed.
 
 end section Security.
 end ORProtocol.
